midterm-project/solutions/host.i.dfy
@@ -1,0 +1,80 @@
+//#title Host protocol
+//#desc Define the host state machine here: message type, state machine for executing one
+//#desc host's part of the protocol.
+
+// Seee exercise01.dfy for an English design of the protocol.
+
+include "network.s.dfy"
+
+module Host {
+  import opened Library
+  import opened HostIdentifiers
+  import Network
+
+  // Define your Message datatype here.
+//#exercise  datatype Message = Message(/* FILL ME IN! */)
+//#start-elide
+  datatype Message = Grant(dest:HostId, epoch:nat)
+//#end-elide
+
+  // Define your Host protocol state machine here.
+  datatype Constants = Constants(myId:HostId) {
+    predicate WF(id:HostId) { // host constants coupled to DistributedSystem Constants.
+      myId == id
+    }
+  }
+//#exercise  datatype Variables = Variables(/* FILL ME IN! */)
+//#start-elide
+  datatype Variables = Variables(holdsLock:bool, epoch:nat)
+//#end-elide
+
+  // DistributedSystem tells us our id so we can recognize inbound messages.
+  predicate Init(c:Constants, v:Variables) {
+//#exercise    true // Replace me
+//#start-elide
+    && v.holdsLock == (c.myId == 0)
+    && v.epoch == if c.myId == 0 then 1 else 0
+//#end-elide
+  }
+
+//#start-elide
+  predicate DoGrant(c:Constants, v:Variables, v':Variables, msgOps:Network.MessageOps<Message>, recipient:HostId) {
+    && v.holdsLock == true
+    && msgOps.recv.None?
+    && ValidHostId(recipient) // Doesn't actually affect safety, but does affect liveness! if we grant to msgOps nonexistent host, no further steps will occur.
+    && msgOps.send == Some(Grant(recipient, v.epoch + 1))
+    && v'.holdsLock == false
+    && v'.epoch == v.epoch
+  }
+
+  predicate DoAccept(c:Constants, v:Variables, v':Variables, msgOps:Network.MessageOps<Message>) {
+    && msgOps.recv.Some?
+    && msgOps.recv.value.dest == c.myId
+    && msgOps.recv.value.epoch > v.epoch
+    && msgOps.send == None
+    && v'.epoch == msgOps.recv.value.epoch
+    && v'.holdsLock == true
+  }
+
+//#end-elide
+  // JayNF
+  datatype Step =
+//#exercise    | SomeStep
+//#start-elide
+    | DoGrantStep(recipient: HostId)
+    | DoAcceptStep
+//#end-elide
+
+  predicate NextStep(c:Constants, v:Variables, v':Variables, msgOps:Network.MessageOps<Message>, step: Step) {
+    match step
+//#exercise       case SomeStep => true
+//#start-elide
+      case DoGrantStep(recipient) => DoGrant(c, v, v', msgOps, recipient)
+      case DoAcceptStep => DoAccept(c, v, v', msgOps)
+//#end-elide
+  }
+
+  predicate Next(c:Constants, v:Variables, v':Variables, msgOps:Network.MessageOps<Message>) {
+    exists step :: NextStep(c, v, v', msgOps, step)
+  }
+}
